theories/theories/utp_theory.thy
@@ -24,21 +24,22 @@ definition WF_THEORY :: "('VALUE ALPHABET set * 'VALUE ALPHA_FUNCTION set) set" 
 "WF_THEORY = {(A,H) | A H . \<forall>a\<in>A. \<forall> hc\<in>H. hc \<in> IDEMPOTENT_OVER a}"
 
 typedef (open) 'VALUE WF_THEORY = "WF_THEORY :: ('VALUE ALPHABET set * 'VALUE ALPHA_FUNCTION set) set"
+  morphisms DestTheory MkTheory
   by (auto simp add:WF_THEORY_def)
 
-declare Rep_WF_THEORY [simp]
-declare Rep_WF_THEORY_inverse [simp]
-declare Abs_WF_THEORY_inverse [simp]
+declare DestTheory [simp]
+declare DestTheory_inverse [simp]
+declare MkTheory_inverse [simp]
 
 setup_lifting type_definition_WF_THEORY
 
 definition utp_alphabets :: 
   "'VALUE WF_THEORY \<Rightarrow> 'VALUE ALPHABET set" ("\<A>") where
-"utp_alphabets t = fst (Rep_WF_THEORY t)"
+"utp_alphabets t = fst (DestTheory t)"
 
 definition healthconds :: 
   "'VALUE WF_THEORY \<Rightarrow> 'VALUE ALPHA_FUNCTION set" ("\<H>") where
-"healthconds t = snd (Rep_WF_THEORY t)"
+"healthconds t = snd (DestTheory t)"
 
 definition THEORY_PRED :: "'VALUE WF_THEORY \<Rightarrow> 'VALUE WF_ALPHA_PREDICATE set" where
 "THEORY_PRED t \<equiv> {p. \<alpha> p \<in> \<A> t \<and> (\<forall> H \<in> \<H> t. p is H healthy)}"
